src/ReactorModel/Objects/Reactor/ReactorType/Basic.lean
@@ -123,61 +123,61 @@ theorem lift_mem_cmp?_ids (cmp) (h : i ∈ (b.cmp? cmp rtr).ids) (hc : cmp ≠ .
 
 end LawfulCoe
 
-inductive Lineage [ReactorType α] (cmp : Component) (i : ID) : α → Type _ 
-  | final : i ∈ (cmp? cmp rtr).ids → Lineage cmp i rtr
-  | nest : (nest rtr₁ j = some rtr₂) → (Lineage cmp i rtr₂) → Lineage cmp i rtr₁
+inductive Member [ReactorType α] (cmp : Component) (i : ID) : α → Type _ 
+  | final : i ∈ (cmp? cmp rtr).ids → Member cmp i rtr
+  | nest : (nest rtr₁ j = some rtr₂) → (Member cmp i rtr₂) → Member cmp i rtr₁
 
-namespace Lineage
+namespace Member
 
 def fromLawfulCoe [ReactorType α] [ReactorType β] [c : LawfulCoe α β] 
-    {rtr : α} {cmp} : (Lineage cmp i rtr) → Lineage cmp i (rtr : β)
+    {rtr : α} {cmp} : (Member cmp i rtr) → Member cmp i (rtr : β)
   | final h  => final (c.lower_mem_cmp?_ids _ h)
-  | nest h l => nest (c.lower_cmp?_eq_some (cmp := .rtr) h) (fromLawfulCoe l)
+  | nest h m => nest (c.lower_cmp?_eq_some (cmp := .rtr) h) (fromLawfulCoe m)
 
 variable [ReactorType α] [ReactorType β] {cmp : Component}
 
-instance [c : LawfulCoe α β] {rtr : α} : Coe (Lineage cmp i rtr) (Lineage cmp i (rtr : β)) where
-  coe := Lineage.fromLawfulCoe
+instance [c : LawfulCoe α β] {rtr : α} : Coe (Member cmp i rtr) (Member cmp i (rtr : β)) where
+  coe := Member.fromLawfulCoe
 
-inductive Equivalent : {rtr₁ : α} → {rtr₂ : β} → (Lineage cmp i rtr₁) → (Lineage cmp i rtr₂) → Prop 
+inductive Equivalent : {rtr₁ : α} → {rtr₂ : β} → (Member cmp i rtr₁) → (Member cmp i rtr₂) → Prop 
   | final : Equivalent (.final h₁) (.final h₂)
-  | nest {n₁ : α} {n₂ : β} {l₁ : Lineage cmp i n₁} {l₂ : Lineage cmp i n₂} :
+  | nest {n₁ : α} {n₂ : β} {m₁ : Member cmp i n₁} {m₂ : Member cmp i n₂} :
     (h₁ : ReactorType.nest rtr₁ j = some n₁) → (h₂ : ReactorType.nest rtr₂ j = some n₂) → 
-    (Equivalent l₁ l₂) → Equivalent (.nest h₁ l₁) (.nest h₂ l₂)
+    (Equivalent m₁ m₂) → Equivalent (.nest h₁ m₁) (.nest h₂ m₂)
 
 namespace Equivalent
 
-theorem symm {rtr₁ : α} {rtr₂ : β} {cmp} {l₁ : Lineage cmp i rtr₁} {l₂ : Lineage cmp i rtr₂}
-    (e : Equivalent l₁ l₂) : (Equivalent l₂ l₁) := by
+theorem symm {rtr₁ : α} {rtr₂ : β} {cmp} {m₁ : Member cmp i rtr₁} {m₂ : Member cmp i rtr₂}
+    (e : Equivalent m₁ m₂) : (Equivalent m₂ m₁) := by
   induction e <;> constructor; assumption
 
 theorem trans 
     [ReactorType γ] {rtr₁ : α} {rtr₂ : β} {rtr₃ : γ}
-    {l₁ : Lineage cmp i rtr₁} {l₂ : Lineage cmp i rtr₂} {l₃ : Lineage cmp i rtr₃}
-    (e₁ : Equivalent l₁ l₂) (e₂ : Equivalent l₂ l₃) : (Equivalent l₁ l₃) := by
-  induction e₁ generalizing l₃ rtr₃ <;> cases e₂ <;> constructor
+    {m₁ : Member cmp i rtr₁} {m₂ : Member cmp i rtr₂} {m₃ : Member cmp i rtr₃}
+    (e₁ : Equivalent m₁ m₂) (e₂ : Equivalent m₂ m₃) : (Equivalent m₁ m₃) := by
+  induction e₁ generalizing m₃ rtr₃ <;> cases e₂ <;> constructor
   case nest.nest hi₁ _ _ _ _ hi₂ => exact hi₁ hi₂
 
 -- Lemma for `to_eq`.
-private theorem to_eq' {rtr₁ rtr₂ : α} {l₁ : Lineage cmp i rtr₁} {l₂ : Lineage cmp i rtr₂} 
-    (h : rtr₁ = rtr₂) (e : Equivalent l₁ l₂) : l₁ = cast (by simp [h]) l₂ := by
+private theorem to_eq' {rtr₁ rtr₂ : α} {m₁ : Member cmp i rtr₁} {m₂ : Member cmp i rtr₂} 
+    (h : rtr₁ = rtr₂) (e : Equivalent m₁ m₂) : m₁ = cast (by simp [h]) m₂ := by
   induction e <;> subst h
   case final => rfl
-  case nest l₁ _ h₁ _ hi h₂ => 
+  case nest m₁ _ h₁ _ hi h₂ => 
     injection h₁ ▸ h₂ with h
     simp [hi h, h]
 
-theorem to_eq {rtr : α} {l₁ l₂ : Lineage cmp i rtr} (e : Equivalent l₁ l₂) : l₁ = l₂ := 
+theorem to_eq {rtr : α} {m₁ m₂ : Member cmp i rtr} (e : Equivalent m₁ m₂) : m₁ = m₂ := 
   e.to_eq' rfl
     
-theorem from_lawfulCoe [LawfulCoe α β] {rtr : α} (l : Lineage cmp i rtr) : 
-    Equivalent l (l : Lineage cmp i (rtr : β)) := by
-  induction l
+theorem from_lawfulCoe [LawfulCoe α β] {rtr : α} (m : Member cmp i rtr) : 
+    Equivalent m (m : Member cmp i (rtr : β)) := by
+  induction m
   case final => constructor
   case nest e => simp [fromLawfulCoe, Equivalent.nest _ _ e]
 
 end Equivalent
-end Lineage
+end Member
 
 class Extensional (α : Type) extends ReactorType α where
   ext_iff : 
@@ -192,12 +192,6 @@ theorem ext [inst : Extensional α] {rtr₁ rtr₂ : α} :
     (ports rtr₁ = ports rtr₂) ∧ (acts rtr₁ = acts rtr₂) ∧ (state rtr₁ = state rtr₂) ∧ 
     (rcns rtr₁ = rcns rtr₂) ∧ (nest rtr₁ = nest rtr₂) → rtr₁ = rtr₂ 
   := inst.ext_iff.mpr
-
-theorem induction [Extensional α] {motive : α → Prop}
-    (base : ∀ rtr, (nest rtr = ∅) → motive rtr)
-    (step : ∀ rtr, (∀ i n, nest rtr i = some n → motive n) → motive rtr) :
-    ∀ rtr, motive rtr :=
-  sorry
 
 instance [ReactorType α] [e : Extensional β] [c : LawfulCoe α β] : Extensional α where
   ext_iff := by
