src/ReactorModel/Objects/Reactor/Core.lean
@@ -47,29 +47,37 @@ theorem insert_cmp?_eq_self {rtr : Reactor.Core} (cmp) {i v} :
   cases cmp <;> try cases ‹Component.Valued› 
   all_goals
     simp [insert, cmp?, reactorType]
-    exact Partial.insert_self_eq _ i v
+    apply Partial.insert_same
 
-theorem insert_cmp?_unchanged {rtr : Reactor.Core} {cmp v} (h : c ≠ cmp ∨ j ≠ i) :
+theorem insert_cmp?_ne_cmp_or_id {rtr : Reactor.Core} {cmp v} (h : c ≠ cmp ∨ j ≠ i) :
     cmp? c rtr j = cmp? c (rtr.insert cmp i v) j := by
-  sorry
+  cases cmp <;> try cases ‹Component.Valued› <;> try cases ‹Kind›
+  all_goals cases c <;> try cases ‹Component.Valued› <;> try cases ‹Kind›
+  all_goals 
+    simp [cmp?, insert]
+    try simp [reactorType]; done
+  all_goals
+    cases h
+    case inl h => contradiction
+    case inr h => exact Partial.insert_ne _ h |>.symm
 
 def updateMem {rtr : Reactor.Core} {cmp : Component.Valued} (f : cmp.type → cmp.type) : 
-    Lineage cmp i rtr → Reactor.Core
+    Member cmp i rtr → Reactor.Core
   | .final h           => rtr.insert cmp i $ f (Partial.mem_ids_iff.mp h).choose
   | .nest (j := j) _ l => rtr.insert .rtr j (updateMem f l)
 
 theorem updateMem_lawfulMemUpdate 
-    {cmp : Component.Valued} (l : Lineage cmp i rtr) 
+    {cmp : Component.Valued} (l : Member cmp i rtr) 
     (f : cmp.type → cmp.type) : LawfulMemUpdate cmp i f rtr (updateMem f l) := by
   induction l <;> simp [updateMem] 
   case final h =>
     replace h := Partial.mem_ids_iff.mp h
-    exact .final insert_cmp?_unchanged h.choose_spec (insert_cmp?_eq_self cmp)
+    exact .final insert_cmp?_ne_cmp_or_id h.choose_spec (insert_cmp?_eq_self cmp)
   case nest h l hi =>
-    exact .nest insert_cmp?_unchanged h (insert_cmp?_eq_self .rtr) hi
+    exact .nest insert_cmp?_ne_cmp_or_id h (insert_cmp?_eq_self .rtr) hi
 
 def update (rtr : Reactor.Core) (cmp : Component.Valued) (i : ID) (f : cmp.type → cmp.type) :=
-  if l : Nonempty (Lineage cmp i rtr) then updateMem f l.some else rtr
+  if l : Nonempty (Member cmp i rtr) then updateMem f l.some else rtr
 
 instance : ReactorType.Updatable Reactor.Core where
   update := update
